Instance.v
@@ -1,17 +1,22 @@
-Require Import Coq.Lists.List. 
+Require Import Coq.Lists.List.  
 Import ListNotations.
 Require Export Cand.
 Require Export Keys.
 Require Export CryptoAxioms.
 Require Export Encryptionschulze.
+Require Export Coq.ZArith.ZArith.
+Require Export Coq.Logic.FinFun.
+Require Export Coq.Program.Basics.
+Require Import Coq.extraction.ExtrOcamlZBigInt.
+Open Scope Z.
 
 (* Create a Cand Instance *)
 Module CndInstance <: Cand.
-  
+
   Inductive Cand := A | B | C.
 
   Definition cand := Cand.
-
+  
   Definition cand_all := [A; B; C].
 
   Lemma cand_fin : forall c, In c cand_all.
@@ -32,9 +37,201 @@ Module CndInstance <: Cand.
 
 End CndInstance.
 
+Module KeyInstance <: Keys.
+
+  Parameter Prime : Type.
+  Parameter prime : Prime. 
+  Extract Constant Prime => "Big.big_int". 
+  Extract Constant prime => "170141183460469231731687303715884114527".
+
+  Parameter Generator : Type.
+  Parameter gen : Generator.
+  Extract Constant Generator => "Big.big_int".
+  Extract Constant gen => "4".
+
+  Parameter Pubkey : Type.
+  Parameter publickey : Pubkey.
+  Extract Constant Pubkey => "Big.big_int".
+  Extract Constant publickey => "49228593607874990954666071614777776087".
+
+  Parameter Prikey : Type.
+  Parameter privatekey : Prikey.
+  Extract Constant Prikey => "Big.big_int".
+  Extract Constant privatekey => "60245260967214266009141128892124363925".
+
+End KeyInstance.
+
+Module AbsInstance.
+
+  Parameter ciphertext : Type.
+  Extract Constant ciphertext => "'ciphertext".
+
+  Parameter Commitment : Type.
+  Extract Constant Commitment => "'commitment".
+
+  (* Permutation Zero Knowledge Proof. *)
+  Parameter PermZkp : Type.
+  Extract Constant PermZkp => "'permZkp".
+
+  (* Randomeness added during the commitment computation *)
+  Parameter S : Type.
+  Extract Constant S => "'s".
+
+  (* Randomeness needed for shuffling the row/column *)
+  Parameter R : Type.
+  Extract Constant R => "'r".
+  
+  (* Zero knowledge proof of Shuffle *)
+  Parameter ShuffleZkp : Type.
+  Extract Constant ShuffleZkp => "'shuffleZkp".
+
+  (* Honest Decryption Zero knowledge Proof *) 
+  Parameter DecZkp : Type.
+  Extract Constant DecZkp => "'decZkp".
+
+End AbsInstance. 
+
+Module CrpInstance <: CryptoAxioms.Crypto CndInstance KeyInstance AbsInstance.
+  Import CndInstance KeyInstance AbsInstance.
+  
+  Definition plaintext := Z.
+
+ 
+    
+  Definition pballot := cand -> cand -> plaintext.
+  
+  Definition eballot := cand -> cand -> ciphertext.
+
+  Definition Group := (Prime * Generator * Pubkey)%type.
+  
+  (*
+  Inductive Group : Type :=
+    group : Prime -> Generator -> Pubkey -> Group. *)
+  
+  (* Construct a instance of group *)
+  Let grp := (prime, gen, publickey).
+
+  (* permutation is Bijective function *)
+  Definition Permutation := existsT (pi : cand -> cand), (Bijective pi).
+
+ 
+  
+  Parameter encrypt_message :
+    Group -> plaintext -> ciphertext.
+  Extract Constant encrypt_message => "Cryptobinding.encrypt_message".
+
+  Parameter decrypt_message :
+    Group -> Prikey -> ciphertext -> plaintext.
+  Extract Constant decrypt_message => "Cryptobinding.decrypt_message".
+
+  (* This function returns zero knowledge proof of encrypted message (c1, c2) *)
+  Parameter construct_zero_knowledge_decryption_proof :
+    Group -> Prikey -> ciphertext -> DecZkp.
+  Extract Constant construct_zero_knowledge_decryption_proof =>
+  "Cryptobinding.construct_zero_knowledge_decryption_proof".
+  
+  (* Unfortunately, this function would not be extract in code, because 
+     it's appears as sort of assertion *)
+  Parameter verify_zero_knowledge_decryption_proof :
+    Group -> plaintext -> ciphertext -> DecZkp -> bool.
+  Extract Constant verify_zero_knowledge_decryption_proof =>
+  "Cryptobinding.verify_zero_knowledge_decryption_proof".
+ 
+  
+  Parameter generatePermutation :
+    Group -> (* group *)
+    nat -> (* length  *)
+    list cand -> (* cand_all *) 
+    Permutation.
+  
+  Extract Constant generatePermutation => 
+  "Cryptobinding.generatePermutation".
 
 
-Module M := Encschulze CndInstance.
+  Parameter generateS : Group -> nat -> S.
+  Extract Constant generateS => "Cryptobinding.generateS".
+  
+  Parameter generatePermutationCommitment :
+    Group -> (* group *)
+    nat -> (* length *)
+    list cand -> (* cand_all *)
+    Permutation -> (* pi *)
+    S -> (*randomness *)
+    Commitment. (* cpi *)
+  Extract Constant generatePermutationCommitment =>
+  "Cryptobinding.generatePermutationCommitment".
+  
 
-Extraction Language Ocaml.
-Extraction "lib.ml" Encshulze.pschulze_winners.
+  (* This function takes Permutation Commitment and S and returns ZKP *)
+  Parameter zkpPermutationCommitment :
+    Group -> (* group *)
+    nat -> (* length *)
+    list cand -> (* cand_all *)
+    Permutation -> (* pi *)
+    Commitment -> (* cpi *)
+    S -> (* randomness *)
+    PermZkp.
+  Extract Constant zkpPermutationCommitment =>
+  "Cryptobinding.zkpPermutationCommitment".
+  
+  Parameter verify_permutation_commitment :
+    Group -> (* group *)
+    nat -> (* length *)
+    Commitment -> (* cpi *)
+    PermZkp -> (* zero knowledge proof *)
+    bool. (* pcps.verify offlineProof offlinePublicInpu *)
+  Extract Constant verify_permutation_commitment =>
+  "Cryptobinding.verify_permutation_commitment".
+    
+  Parameter homomorphic_addition :
+    Group -> ciphertext -> ciphertext -> ciphertext.
+  Extract Constant homomorphic_addition => "Cryptobinding.homomorphic_addition".
+  
+  Parameter generateR : Group -> nat -> R.
+  Extract Constant generateR => "Cryptobinding.generateR".
+  
+  Parameter shuffle :
+    Group -> (* group *)
+    nat -> (* Length of list cand *)
+    list cand -> (* cand_all because we need to convert function into list *)
+    (forall n m : cand, {n = m} + {n <> m}) -> (* This is need because we want to construct the ballot *)
+    (cand -> ciphertext) -> (* ciphertext *)
+    Permutation -> (* pi *)
+    R -> (* Randomness R *)
+    (cand -> ciphertext).
+  Extract Constant shuffle => "Cryptobinding.shuffle".
+
+  
+  Parameter shuffle_zkp :
+    Group -> (* group *)
+    nat -> (* length *)
+    list cand -> (* cand_all *)
+    (cand -> ciphertext) -> (* cipertext *)
+    (cand -> ciphertext) -> (* shuffle cipertext *)
+    Permutation -> (* pi *)
+    Commitment -> (* cpi *)
+    S -> (* s, permutation commitment randomness *)
+    R -> (* r, shuffle randomness *)
+    ShuffleZkp. (* zero knowledge proof of shuffle *)
+  Extract Constant shuffle_zkp => "Cryptobinding.shuffle_zkp".
+  
+  Parameter verify_shuffle:
+    Group -> (* group *)
+    nat -> (* length *)
+    list cand ->
+    (cand -> ciphertext) -> (* cipertext *)
+    (cand -> ciphertext) -> (* shuffled cipertext *)
+    Commitment -> (* permutation commitment *)
+    ShuffleZkp -> (* zero knowledge proof of shuffle *)
+    bool. (* true or false *)
+  Extract Constant verify_shuffle => "Cryptobinding.verify_shuffle".
+
+End CrpInstance.
+ 
+Module M := Encschulze CndInstance KeyInstance AbsInstance CrpInstance.
+
+Extraction Language OCaml.
+(* Avoid name clash with modules *)
+Extraction Blacklist List String Int.
+Separate Extraction M.pschulze_winners.
+
