Makefile
@@ -26,6 +26,17 @@ CryptoWrapper : schulze/CryptoWrapper.class
 jarfile : schulze/CryptoWrapper.class
 		jar cvf schulze/schulze.jar schulze/CryptoWrapper.class
 
+
+Main : main.ml
+	ocamlfind ocamlopt -O3 -o a.out -linkpkg -package str,num,menhirLib -I ocaml-java/bin/camljava camljava.cmxa -ppx ocaml-java/bin/ocaml-java-ppx parser.mli parser.ml big.ml lexer.ml \
+		Sumbool.mli Sumbool.ml Cand.mli Cand.ml Keys.mli Keys.mli Specif.ml Datatypes.mli Datatypes.ml BinPos.mli BinPos.ml BinInt.mli BinInt.ml CryptoAxioms.mli CryptoAxioms.ml List0.mli List0.ml  \
+		PeanoNat.mli PeanoNat.ml ZArith_dec.mli ZArith_dec.ml Zbool.mli Zbool.ml ListLemma.mli ListLemma.ml ValidityExist.ml  ZArith_dec.mli ZArith_dec.ml cryptobinding.ml Schulze.mli \
+		Schulze.ml Encryptionschulze.mli Encryptionschulze.ml Top.ml main.ml
+
+
 #clean 
 clean:
-	rm -rf _build *.vo *.glob *.class *.cmi *.cmx *.o *.out lib.ml lib.mli main.native main.byte schulze/*.class schulze/*.jar 2>/dev/null || true
+	rm -rf _build *.vo *.glob *.class *.cmi *.cmx *.o *.out BinInt.* BinNums.* BinPos.* Cand.ml Cand.mli  CryptoAxioms.ml CryptoAxioms.mli \
+		Datatypes.ml Datatypes.mli Encryptionschulze.ml Encryptionschulze.mli Keys.ml Keys.mli ListLemma.ml ListLemma.mli List.ml \
+		List.mli PeanoNat.ml PeanoNat.mli Schulze.ml Schulze.mli Specif.ml Specif.mli  Sumbool.ml  Sumbool.mli Top.ml Top.mli \
+		ValidityExist.ml ValidityExist.mli ZArith_dec.ml ZArith_dec.mli Zbool.ml Zbool.mli lib.ml lib.mli main.native main.byte schulze/*.class schulze/*.jar 2>/dev/null || true
